# F29

## F29-2: Gaussian Elimination

### Linear Equation System

$\begin{cases} - x_2 - x_3 = -1 \\ - x_1 + 2 x_2 + x_3 = 0 \\ 3 x_1 - x_2 + 2 x_3 = 5 \end{cases}$

$\leftrightarrow \begin{bmatrix} 0 & -1 & -1 \\ -1 & 2 & 1 \\ 3 & 1 & 2 \end{bmatrix}
\begin{bmatrix} x_1 \\ x_2 \\ x_3 \end{bmatrix}
=
\begin{bmatrix} -1 \\ 0 \\ 5 \end{bmatrix}$

$\leftrightarrow
\begin{bmatrix} 1 & 0 & 1 \\ 0 & 1 & 1 \\ 0 & 0 & 0 \end{bmatrix}
\begin{bmatrix} x_1 \\ x_2 \\ x_3 \end{bmatrix}
=
\begin{bmatrix} 2 \\ 1 \\ 0 \end{bmatrix}
$

$\leftrightarrow \begin{cases}x_1 + x_3 = 2 \\ x_2 + x_3 = 1 \end{cases}$

$\leftrightarrow \begin{cases}x_1 = 2 - x_3 \\ x_2 = 1 - x_3 \end{cases}$

$x = \begin{bmatrix} x_1 \\  x_2 \\ x_3 \end{bmatrix}
= \begin{bmatrix} 2 - x_3 \\ 1 - x_3 \\ x_3 \end{bmatrix}
= \begin{bmatrix} 2 \\ 1 \\ 0 \end{bmatrix}
+ \begin{bmatrix} - x_3 \\ - x_3 \\ x_3 \end{bmatrix}
= \begin{bmatrix} 2 \\ 1 \\ 0 \end{bmatrix}
+ \begin{bmatrix} -1 \\ -1 \\ 1 \end{bmatrix}t $

### Inverse Matrix

*Q. Find the inverse matrix of* $\begin{bmatrix} 1 & 2 & 3 \\ 2 & 3 & 5 \\ 1 & 0 & 2 \end{bmatrix}$.

$
  \left[\begin{array}{rrr|rrr}
    1 & 2 & 3 & 1 & 0 & 0 \\
    2 & 3 & 5 & 0 & 1 & 0 \\
    1 & 0 & 2 & 0 & 0 & 1
  \end{array}\right]
$

$\leftrightarrow 
  \left[\begin{array}{rrr|rrr}
    1 & 2 & 3 & 1 & 0 & 0 \\
    0 & -1 & -1 & -2 & 1 & 0 \\
    0 & -2 & -1 & -1 & 0 & 1
  \end{array}\right]
$

$\leftrightarrow 
  \left[\begin{array}{rrr|rrr}
    1 & 2 & 3 & 1 & 0 & 0 \\
    0 & 1 & 1 & 2 & -1 & 0 \\
    0 & -2 & -1 & -1 & 0 & 1
  \end{array}\right]
$

$\leftrightarrow 
  \left[\begin{array}{rrr|rrr}
    1 & 2 & 3 & 1 & 0 & 0 \\
    0 & 1 & 1 & 2 & -1 & 0 \\
    0 & 0 & 1 & 3 & -2 & 1
  \end{array}\right]
$

$\leftrightarrow 
  \left[\begin{array}{rrr|rrr}
    1 & 2 & 0 & -8 & 6 & -3 \\
    0 & 1 & 0 & -1 & 1 & -1 \\
    0 & 0 & 1 & 3 & -2 & 1
  \end{array}\right]
$

$\leftrightarrow 
  \left[\begin{array}{rrr|rrr}
    1 & 0 & 0 & -6 & 4 & -1 \\
    0 & 1 & 0 & -1 & 1 & -1 \\
    0 & 0 & 1 & 3 & -2 & 1
  \end{array}\right]
$

$\therefore {\begin{bmatrix} 1 & 2 & 3 \\ 2 & 3 & 5 \\ 1 & 0 & 2 \end{bmatrix}}^{-1} = 
\begin{bmatrix} -6 & 4 & -1 \\ -1 & 1 & -1 \\ 0 & 0 & 1 \end{bmatrix}
$

---

## F29-7: Eigen decomposition

*Q. Diagonalize the matrix*
$A = \begin{bmatrix} 1 & -3 & 3 \\ 0 & -5 & 6 \\ 0 & -3 & 4 \end{bmatrix}$.

$
\lambda I - A = \begin{bmatrix} 
\lambda - 1 & 3 & -3 \\ 0 & \lambda + 5 & -6 \\ 0 & 3 & \lambda - 4 
\end{bmatrix}
$

$
\det (\lambda I - A) = 
(\lambda - 1) \det \begin{bmatrix} 
\lambda + 5 & -6 \\ 3 & \lambda -4 \end{bmatrix} 
- 3 \det \begin{bmatrix} 0 & -6 \\ 0 & \lambda -4 \end{bmatrix}
+ (-3) \det \begin{bmatrix} 0 & \lambda + 5 \\ 0 & 3 
\end{bmatrix}
$

$
= (\lambda - 1)((\lambda + 5)(\lambda - 4) + 18) - 3*0 + (-3)*0
$

$
= (\lambda - 1)^2 (\lambda + 2)
$

$
= 0
$

$
\therefore \lambda_1 = 1, \lambda_2 = 1, \lambda_3 = -2
$

i) $\lambda = 1$

$
\lambda I - A = \begin{bmatrix}
0 & 3 & -3 \\ 0 & 6 & -6 \\ 0 & 3 & -3
\end{bmatrix}
$

$
B_1 = 
\begin{bmatrix} 0 & 3 & -3 \\ 0 & 6 & -6 \\ 0 & 3 & -3 \end{bmatrix}
\begin{bmatrix} x_1 \\ x_2 \\ x_3 \end{bmatrix}
=0
$

$ \leftrightarrow
\begin{cases}
3 x_2 -3 x_3 = 0 \\
6 x_2 -6 x_3 = 0 \\
3 x_2 -3 x_3 = 0
\end{cases}
$

$\leftrightarrow x_2 = x_3$

$
\begin{bmatrix} x_1 \\ x_2 \\ x_3 \end{bmatrix}
= \begin{bmatrix} x_1 \\ x_2 \\ x_2 \end{bmatrix}
= \begin{bmatrix} x_1 \\ 0 \\ 0 \end{bmatrix} + \begin{bmatrix} 0 \\ x_2 \\ x_2 \end{bmatrix}
= \begin{bmatrix} 1 \\ 0 \\ 0 \end{bmatrix} t + \begin{bmatrix} 0 \\ 1 \\ 1 \end{bmatrix} s
$

$ \therefore
v_1 = 
\begin{bmatrix}
1 \\ 0 \\ 0
\end{bmatrix}
,
v_2 = 
\begin{bmatrix}
0 \\ 1 \\ 1
\end{bmatrix}
$

ii) $\lambda = -2$

$
\lambda I - A = \begin{bmatrix}
-3 & 3 & -3 \\ 0 & 3 & -6 \\ 0 & 3 & -6
\end{bmatrix}
$

$
B_2 = 
\begin{bmatrix} -3 & 3 & -3 \\ 0 & 3 & -6 \\ 0 & 3 & -6 \end{bmatrix}
\begin{bmatrix} x_1 \\ x_2 \\ x_3 \end{bmatrix}
= 0
$

$ \leftrightarrow
\begin{cases}
-3 x_1 +3 x_2 -3 x_3 = 0 \\
3 x_2 -6 x_3 = 0 \\
3 x_2 -6 x_3 = 0
\end{cases}
$

$\leftrightarrow x_1 = x_3 , 2 x_2 = x_3 $

$
\begin{bmatrix}
x_1 \\ x_2 \\ x_3
\end{bmatrix}
=
\begin{bmatrix}
x_3 \\ 2 x_3 \\ x_3
\end{bmatrix}
=
\begin{bmatrix}
1 \\ 2 \\ 1
\end{bmatrix}
t
$

$ \therefore
v_3 = 
\begin{bmatrix}
1 \\ 2 \\ 1
\end{bmatrix}
$

$
Q = 
\begin{bmatrix} v_1 & v_2 & v_3 \end{bmatrix}
= \begin{bmatrix} 1 & 0 & 1 \\ 0 & 1 & 2 \\ 0 & 1 & 1 \end{bmatrix}
$

$Q^{-1} = \begin{bmatrix} 1 & -1 & 1 \\ 0 & -1 & 2 \\ 0 & 1 & -1 \end{bmatrix}$

$\therefore D = Q^{-1}AQ = 
\begin{bmatrix} 1 & -1 & 1 \\ 0 & -1 & 2 \\ 0 & 1 & 3 \end{bmatrix}
\begin{bmatrix} 1 & -3 & 3 \\ 0 & -5 & 6 \\ 0 & -3 & 4 \end{bmatrix}
\begin{bmatrix} 1 & 0 & 1 \\ 0 & 1 & 2 \\ 0 & 1 & 1 \end{bmatrix}
=
\begin{bmatrix} 1 & 0 & 0 \\ 0 & 1 & 0 \\ 0 & 0 & -2 \end{bmatrix}
$

---

## F29-8: Singular Value Decomposition

*Q. Find the SVD of* 
$A = \begin{bmatrix} 1.2 & 0.9 & -4 \\ 1.6 & 1.2 & 3 \end{bmatrix}$.

$
AA^T = \begin{bmatrix} 1.2 & 0.9 & -4 \\ 1.6 & 1.2 & 3 \end{bmatrix}
\begin{bmatrix} 1.2 & 1.6 \\ 0.9 & 1.2 \\ -4 & 3 \end{bmatrix}
= \begin{bmatrix} 18.25 & -9 \\ -9 & 13 \end{bmatrix}
$

$
\lambda I- AA^T = \begin{bmatrix} \lambda - 18.25 & 9 \\ 9 & \lambda - 13 \end{bmatrix}
$

$\det (\lambda I - AA^T) = (\lambda - 18.25)(\lambda - 13) - 81$

$= \lambda^2 - 31.25 \lambda + 156.25$

$ = (\lambda - 25)(4\lambda - 25) $


$=0 $

$\therefore \lambda_1 = 25, \lambda_2 = 6.25$

i) $\lambda = 25$

$
\lambda I - AA^T = \begin{bmatrix} 6.75 & 9 \\ 9 & 12 \end{bmatrix}
$

$
B_1 = \begin{bmatrix} 6.75 & 9 \\ 9 & 12 \end{bmatrix}
\begin{bmatrix} x_1 \\ x_2 \end{bmatrix}
= 0
$

$ \leftrightarrow
\begin{cases} 6.75 x_1 + 9 x_2 = 0 \\ 9 x_1 + 12 x_2 = 0 \end{cases}
$

$\leftrightarrow
3 x_1 = -4 x_2
$

$
\begin{bmatrix} x_1 \\ x_2 \end{bmatrix}
= \begin{bmatrix} x_1 \\ -\frac{3}{4} x_1 \end{bmatrix}
= \begin{bmatrix} -0.8 \\ 0.6 \end{bmatrix} t
$

$\therefore u_1 = \begin{bmatrix} -0.8 \\ 0.6 \end{bmatrix}$

ii) $\lambda =  6.25$

$
\lambda I - AA^T = \begin{bmatrix} -12 & 9 \\ 9 & -6.75 \end{bmatrix}
$

$
B_2 = \begin{bmatrix} -12 & 9 \\ 9 & -6.75 \end{bmatrix}
= \begin{bmatrix} x_1 \\ x_2 \end{bmatrix}
= 0
$

$ \leftrightarrow
\begin{cases} -12 x_1 + 9 x_2 = 0 \\ 9 x_1 + -6.75 x_2 = 0 \end{cases}
$

$\leftrightarrow
4 x_1 = 3 x_2
$

$
\begin{bmatrix} x_1 \\ x_2 \end{bmatrix}
= \begin{bmatrix} x_1 \\ \frac{4}{3} x_1 \end{bmatrix}
= \begin{bmatrix} 0.6 \\ 0.8 \end{bmatrix} t
$

$\therefore u_2 = \begin{bmatrix} 0.6 \\ 0.8 \end{bmatrix}$

$
A^T A = 
\begin{bmatrix} 1.2 & 1.6 \\ 0.9 & 1.2 \\ -4 & 3 \end{bmatrix}
\begin{bmatrix} 1.2 & 0.9 & -4 \\ 1.6 & 1.2 & 3 \end{bmatrix}
= \begin{bmatrix} 4 & 3 & 0 \\ 3 & 2.25 & 0 \\ 0 & 0 & 25 \end{bmatrix}
$

$
\lambda I - A^T A =
\begin{bmatrix} \lambda -4 & -3 & 0 \\ -3 & \lambda -2.25 & 0 \\ 0 & 0 & \lambda -25 \end{bmatrix}
$

$
\det (\lambda - A^T A) =
(\lambda - 4) \det \begin{bmatrix} \lambda - 2.25 & 0 \\ 0 & \lambda - 25 \end{bmatrix}
- (-3) \det \begin{bmatrix} -3 & 0 \\ 0 & \lambda - 25 \end{bmatrix}
+ 0 \det \begin{bmatrix} -3 & \lambda - 2.25 \\ 0 & 0 \end{bmatrix}
$

$= (\lambda - 4)(\lambda - 2.25)(\lambda - 25) + 3 * (-3) (\lambda - 25) + 0$

$= \lambda(\lambda - 6.25)(\lambda - 25)$

$= 0$

$\therefore \lambda_1 = 25, \lambda_2 = 6.25, \lambda_3 = 0, \sigma_1 = 5, \sigma_2 = 2.5$

i) $\lambda = 25$

$
\lambda I - A^T A = \begin{bmatrix} 21 & -3 & 0 \\ -3 & 22.75 & 0 \\ 0 & 0 & 0 \end{bmatrix}
$

$
B_1 = \begin{bmatrix} 21 & -3 & 0 \\ -3 & 22.75 & 0 \\ 0 & 0 & 0 \end{bmatrix}
\begin{bmatrix} x_1 \\ x_2 \\ x_3 \end{bmatrix} = 0
$

$ \leftrightarrow
\begin{cases} 21 x_1 -3 x_2 = 0 \\ -3 x_1 +22.75 x_2 = 0 \end{cases}
$

$\leftrightarrow x_1 = x_2 = 0$

$
\begin{bmatrix} x_1 \\ x_2 \\ x_3 \end{bmatrix}
= \begin{bmatrix} 0 \\ 0 \\ x_3 \end{bmatrix}
= \begin{bmatrix} 0 \\ 0 \\ 1 \end{bmatrix} t
$

$\therefore v_1 = \begin{bmatrix} 0 \\ 0 \\ 1 \end{bmatrix} $

ii) $\lambda = 6.25$

$
\lambda I - A^T A = \begin{bmatrix} 2.25 & -3 & 0 \\ -3 & 4 & 0 \\ 0 & 0 & -18.75 \end{bmatrix}
$

$
B_2 = \begin{bmatrix} 2.25 & -3 & 0 \\ -3 & 4 & 0 \\ 0 & 0 & -18.75 \end{bmatrix}
\begin{bmatrix} x_1 \\ x_2 \\ x_3 \end{bmatrix} = 0
$

$ \leftrightarrow
\begin{cases} 2.25 x_1 - 3 x_2 = 0 \\ -3 x_1 + 4 x_2 = 0 \\ -18.75 x_3 = 0 \end{cases}
$

$ \leftrightarrow
\begin{cases} 3 x_1 = 4 x_2 \\ x_3 = 0 \end{cases}
$

$
\begin{bmatrix} x_1 \\ x_2 \\ x_3 \end{bmatrix}
= \begin{bmatrix} x_1 \\ \frac{3}{4}x_1 \\ 0 \end{bmatrix}
= \begin{bmatrix} 0.8 \\ 0.6 \\ 0 \end{bmatrix}t
$

$ \therefore v_2 = \begin{bmatrix} 0.8 \\ 0.6 \\ 0 \end{bmatrix} $

iii) $\lambda = 0$

$
\lambda I - A^T A = \begin{bmatrix} -4 & -3 & 0 \\ -3 & -2.25 & 0 \\ 0 & 0 & -25 \end{bmatrix}
$

$
B_3 = \begin{bmatrix} -4 & -3 & 0 \\ -3 & -2.25 & 0 \\ 0 & 0 & -25 \end{bmatrix}
\begin{bmatrix} x_1 \\ x_2 \\ x_3 \end{bmatrix} = 0
$

$ \leftrightarrow
\begin{cases} -4 x_1 - 3 x_2 = 0 \\ -3 x_1 - 2.25 x_2 = 0 \\ -25 x_3 = 0 \end{cases}
$

$ \leftrightarrow
\begin{cases} 4 x_1 = -3 x_2 \\ x_3 = 0 \end{cases}
$

$
\begin{bmatrix} x_1 \\ x_2 \\ x_3 \end{bmatrix}
= \begin{bmatrix} x_1 \\ -\frac{4}{3}x_1 \\ 0 \end{bmatrix}
= \begin{bmatrix} -0.6 \\ 0.8 \\ 0 \end{bmatrix} t
$

$ \therefore v_3 = \begin{bmatrix} -0.6 \\ 0.8 \\ 0 \end{bmatrix} $

$ \therefore
A = U \Sigma V^T  = 
\begin{bmatrix} u_1 & u_2 \end{bmatrix} 
\begin{bmatrix} \sigma_1 & 0 & 0 \\ 0 & \sigma_2 & 0 \\ 0 & 0 & 0 \end{bmatrix} 
\begin{bmatrix} v_1 ^T \\ v_2 ^T \\ v_3 ^T \end{bmatrix}
= 
\begin{bmatrix} -0.8 & 0.6 \\ 0.6 & 0.8 \end{bmatrix} 
\begin{bmatrix} 5 & 0 & 0 \\ 0 & 2.5 & 0 \\ 0 & 0 & 0 \end{bmatrix} 
\begin{bmatrix} 0 & 0 & 1 \\ 0.8 & 0.6 & 0 \\ -0.6 & 0.8 & 0 \end{bmatrix}
$

---

## F29-10: Gradient vector, Directional Derivative

*Get a tangent line of the ellipse* $\frac{x^2}{4}+y^2 = 2$ *at* $(-2,1)$ *using gradient vector*.

$
\nabla f = (f_x, f_y) = (\frac{1}{2}x, 2y)
$

$\nabla f (-2, 1) = (-1, 2)$

$\therefore l = -(x+2)+2(y-1)=0$
